Update Theories

isabelle/Correspondence.thy
@@ -2,70 +2,121 @@ theory Correspondence
   imports Invariants Summaries
 begin
 
-(* Corollary: Coincidence of Invariants and Summaries
-   proof via soundness and completeness of the approaches *)
+(* Not explicitly stated in the paper
+   but mirrors Corollary 1 below. *)
+corollary invariant_adequate:
+  "hoare P (while t B) Q
+     \<longleftrightarrow> (\<exists> I.   invariant_safe P I t B
+               \<and> invariant_correct P I t B Q)"
+  by (meson invariant_complete invariant_sound)
+
+(* Definition 5: (Correct) Loop Contracts *)
+definition contract_correct :: "'a cond \<Rightarrow> 'a cond \<Rightarrow> 'a cond \<Rightarrow> 'a prog \<Rightarrow> 'a rel \<Rightarrow> 'a cond \<Rightarrow> bool"
+  where
+"contract_correct P I t B R Q
+  \<equiv>   invariant_safe P I t B
+    \<and> summary_correct P t B R Q"
+
+(* Corollary 1: Adequacy of Loop Contracts *)
+corollary contract_adequate:
+  "hoare P (while t B) Q
+    \<longleftrightarrow> (\<exists> I R. contract_correct P I t B R Q)"
+  by (meson contract_correct_def hoare_split invariant_safe invariant_adequate summary_complete summary_correct)
+
+(* Corollary 2: Coincidence of Invariants and Summaries
+
+   Proof via soundness and completeness of the approaches,
+   check coincidence' below for a proof using the syntactic translations.
+
+   Note, we do not bother here to add safe invariants
+   (i.e., formulate the corollary with contracts)
+   as it is plain obvious. *)
 corollary coincidence:
   "(\<exists> I. invariant_correct P I t B Q)
     \<longleftrightarrow> (\<exists> R. summary_correct P t B R Q)"
   by (metis (lifting) invariant_correct invariant_correct_complete summary_correct summary_complete)
 
-(* Proposition 1: Lifting of Summaries to Invariants *)
+(* Proposition 1: Invariants from Contracts
+
+   We prove two versions, one for just correctness,
+   and one that includes safety as well (which is shown in the paper) *)
 proposition lift_summary:
   assumes "summary_correct   P t B R Q"
-  shows   "invariant_correct P (\<lambda> s0 s. P s0 \<and> (\<forall> sn. R s sn \<longrightarrow> R s0 sn)) t B Q"
+  shows   "invariant_correct P (\<lambda> s. \<exists> s0. P s0 \<and> (\<forall> sn. R s sn \<longrightarrow> R s0 sn)) t B Q"
+  using assms by rule blast
+
+proposition lift_contract:
+  assumes "contract_correct  P J t B R Q"
+  shows   "invariant_safe    P (\<lambda> s. \<exists> s0. P s0 \<and> J s \<and> (\<forall> sn. R s sn \<longrightarrow> R s0 sn)) t B"
+    and   "invariant_correct P (\<lambda> s. \<exists> s0. P s0 \<and> J s \<and> (\<forall> sn. R s sn \<longrightarrow> R s0 sn)) t B Q"
+proof -
+  show "invariant_safe    P (\<lambda> s. \<exists> s0. P s0 \<and> J s \<and> (\<forall> sn. R s sn \<longrightarrow> R s0 sn)) t B"
+  proof (rule, goal_cases)
+    case (1 s0)
+    then show ?case
+      using assms unfolding contract_correct_def by blast
+  next
+    case (2 s s')
+    (* The automatic proof tactics (blast, ...)
+       choke on the existential quantifier
+       and on propagating J from s to s' *)
+    from 2(1) obtain s0 where "P s0" "J s" "\<And> sn. R s sn \<Longrightarrow> R s0 sn"
+      by blast
+    with 2(2,3) have "P s0 \<and> J s' \<and> (\<forall>sn. R s' sn \<longrightarrow> R s0 sn)"
+      using assms unfolding contract_correct_def by blast
+    then show ?case ..
+  next
+    case (3 s)
+    then show ?case
+      using assms unfolding contract_correct_def by blast
+  qed
+next
+  show "invariant_correct P (\<lambda> s. \<exists> s0. P s0 \<and> J s \<and> (\<forall> sn. R s sn \<longrightarrow> R s0 sn)) t B Q"
+  proof (rule, goal_cases)
+    case (1 s0)
+    then show ?case
+      using assms unfolding contract_correct_def by blast
+  next
+    case (2 s s') (* same as above *)
+    from 2(1) obtain s0 where "P s0" "J s" "\<And> sn. R s sn \<Longrightarrow> R s0 sn"
+      by blast
+    with 2(2,3) have "P s0 \<and> J s' \<and> (\<forall>sn. R s' sn \<longrightarrow> R s0 sn)"
+      using assms unfolding contract_correct_def by blast
+    then show ?case ..
+  next
+    case (3 s)
+    then show ?case
+      using assms unfolding contract_correct_def by blast
+  next
+    case (4 s s')
+    then show ?case
+      using assms unfolding contract_correct_def by blast
+  qed
+qed
+
+(* Proposition 2: Contracts from Invariants
+
+   Again, we prove a simple version for correctness,
+   and one for full contracts, for the formulation with break.
+
+   See Simple.thy for a variant without breaks/runtime errors. *)
+proposition lift_invariant:
+  assumes "invariant_correct P I t B Q"
+  shows   "summary_correct   P t B (\<lambda> s sn. I s \<longrightarrow> Q sn) Q"
   using assms by blast
 
-(* Proposition 2: Lifting of Postconditions to Summaries *)
-proposition lift_post:
+proposition lift_invariant':
+  assumes "invariant_safe    P I t B"
   assumes "invariant_correct P I t B Q"
-  shows   "summary_correct   P t B (\<lambda> s sn. \<forall> s0. I s0 s \<longrightarrow> Q sn) Q"
-  using assms by blast
+  shows   "contract_correct  P I t B (\<lambda> s sn. I s \<longrightarrow> Q sn) Q"
+  using assms unfolding contract_correct_def by blast
 
 (* Corollary 2: Coincidence of Invariants and Summaries
-   proof using the constructure translation *)
+   proof using the constructive translation *)
 corollary coincidence':
   "(\<exists> I. invariant_correct P I t B Q)
     \<longleftrightarrow> (\<exists> R. summary_correct P t B R Q)"
-  by (metis (lifting) lift_summary lift_post)
+  by (metis (lifting) lift_summary lift_invariant)
 
-(* Soundness of a "stronger" formulation that includes preconditions and invariants in the conditions for summaries,
-   all in one large set of proof obligations. *)
-inductive combined :: "'a cond \<Rightarrow> 'a rel \<Rightarrow> 'a cond \<Rightarrow> 'a prog \<Rightarrow> 'a rel \<Rightarrow> 'a cond \<Rightarrow> bool" where
-combinedI[intro!]:
-"\<lbrakk>\<And> s0.         \<lbrakk>P s0\<rbrakk> \<Longrightarrow> I s0 s0;
-  \<And> s0 s s'.    \<lbrakk>P s0; I s0 s; t s; B s (Ok s')\<rbrakk> \<Longrightarrow> I s0 s';
- 
-  \<And> s0 s.       \<lbrakk>P s0; I s0 s; t s; B s Err\<rbrakk> \<Longrightarrow> False;
-  
-  \<And> s0 s.       \<lbrakk>P s0; I s0 s; \<not> t s\<rbrakk> \<Longrightarrow> R s s;
-  \<And> s0 s s'.    \<lbrakk>P s0; I s0 s; t s; B s (Brk s')\<rbrakk> \<Longrightarrow> R s s';
-  \<And> s0 s s' sn. \<lbrakk>P s0; I s0 s; t s; R s' sn; B s (Ok s')\<rbrakk> \<Longrightarrow> R s sn;
-
-  \<And> s0 sn.   \<lbrakk>P s0; R s0 sn\<rbrakk> \<Longrightarrow> Q sn\<rbrakk>
-  \<Longrightarrow> combined P I t B R Q"
-
-inductive_cases combinedE[elim!]: "combined P I t B R Q"
-
-(* Soundness of the combined approach,
-   via safe invariants,
-   and one of either correct invariants or correct summaries *)
-
-lemma combined_invariant_safe:
-  assumes "combined P I t B R Q"
-  shows   "invariant_safe P (\<lambda> s0 s. P s0 \<and> I s0 s) t B"
-  using assms by blast
-
-lemma combined_invariant_correct:
-  assumes "combined P I t B R Q"
-  shows   "invariant_correct P (\<lambda> s0 s. P s0 \<and> I s0 s \<and> (\<forall> sn. R s sn \<longrightarrow> R s0 sn)) t B Q"
-  using assms
-  apply (elim combinedE)
-  apply (intro invariant_correctI)
-  by meson+
-
-lemma combined_summary_correct:
-  assumes "combined P I t B R Q"
-  shows   "summary_correct P t B (\<lambda> s sn. \<forall> s0. P s0 \<and> I s0 s \<longrightarrow> R s sn) Q"
-  using assms by blast
 
 end
