isabelle/Rules.thy
@@ -1,0 +1,100 @@
+theory Rules
+  imports Correspondence
+begin
+
+lemma hoare_conseq:
+  assumes "hoare P' c Q'"
+  assumes "\<And> s. P  s \<Longrightarrow> P' s"
+  assumes "\<And> s. Q' s \<Longrightarrow> Q  s"
+  shows   "hoare P  c Q"
+  using assms by blast
+
+lemma hoare_spec:
+  shows   "hoare P (spec P R) (\<lambda> s. \<exists> s0. P s0 \<and> R s0 s)"
+  by rule auto
+
+lemma spec_conseq:
+  assumes "hoare P (spec I R) Q"
+  shows   "\<And> s. P s \<Longrightarrow> I s"
+          "\<And> s0 s. P s0 \<and> R s0 s \<Longrightarrow> Q s"
+proof -
+  fix s
+  assume P: "P s"
+  from assms show "I s"
+  proof (elim hoareE)
+    from P show "P s" .
+  next
+    show "spec I R s (Ok s)"
+      apply simp
+
+
+
+lemma hoare_seq:
+  assumes "hoare P c1 Q"
+  assumes "hoare Q c2 R"
+  shows   "hoare P (seq c1 c2) R"
+  using assms by (auto elim!: seqE)
+
+(* Definition 2: Validity of Hoare-Triples (partial correctness *)
+inductive hoare' :: "'a cond \<Rightarrow> 'a prog \<Rightarrow> 'a cond \<Rightarrow> 'a cond \<Rightarrow> bool" where
+hoare'I[intro!]:
+"\<lbrakk>\<And> s r. P s \<Longrightarrow> c s r \<Longrightarrow> (\<exists> s'. r = Brk s' \<and> B s') \<or> (\<exists> s'. r = Ok s' \<and> Q s')\<rbrakk>
+  \<Longrightarrow> hoare' P c B Q"
+
+inductive_cases hoare'E[elim!]: "hoare' P c B Q"
+
+lemma hoare':
+  "hoare' P c (\<lambda> s. False) Q \<longleftrightarrow> hoare P c Q"
+  by blast
+
+
+lemma hoare_invariant:
+  assumes "hoare P skip I"
+  assumes "hoare  (\<lambda> s. \<not> t s \<and> I s) skip Q"
+  assumes "hoare' (\<lambda> s. t s \<and> I s) B Q I"
+  shows   "hoare P (while t B) Q"
+  apply (rule invariant_sound[where ?I = "I"])
+  sorry
+  
+
+lemma hoare_contract:
+  assumes "hoare P (spec I R) Q"
+  assumes "\<And> sn. hoare  (\<lambda> s. \<not> t s \<and> I s \<and> sn = s) skip (\<lambda> s. R sn s)"
+  assumes "\<And> si. hoare  (\<lambda> s.   t s \<and> I s \<and> si = s) (seq B (spec I R)) (\<lambda> s. R si s)"
+  shows   "hoare P (while t B) Q"
+  apply (rule combined_sound[where ?I = "I" and ?R = "R"])
+proof (rule, goal_cases)
+  case (1 s0)
+  then show ?case
+    using assms(1) by auto
+next
+  case (2 s s')
+  then show ?case
+    using assms(3)[of s] by (auto elim!: hoareE)
+next
+  case (3 s)
+  then show ?case
+    using assms(3)[of s] by (auto elim!: hoareE)
+next
+  case (4 s)
+  then show ?case
+    using assms(2)[of s] by (auto elim!: hoareE)
+next
+  case (5 s s')
+  then show ?case
+    using assms(3)[of s] by (auto elim!: hoareE)
+next
+  case (6 s s' sn)
+  then have "I s'"
+    using assms(3)[of s] by (auto elim!: hoareE)
+  with 6 show ?case
+    using assms(3)[of s] by (auto elim!: hoareE intro!: seq_Ok)
+next
+  case (7 s0 sn)
+  from 7 have "I s0"
+    using assms(1) by auto
+  with 7 show ?case
+    using assms(1) by (auto elim!: hoareE)
+qed
+
+end
