isabelle/Simple.thy
@@ -1,0 +1,315 @@
+theory Simple
+  imports Main
+begin
+
+type_synonym 'a cond = "'a \<Rightarrow> bool"
+type_synonym 'a rel  = "'a \<Rightarrow> 'a \<Rightarrow> bool"
+type_synonym 'a prog = "'a \<Rightarrow> 'a \<Rightarrow> bool"
+
+(* Definition 1: Semantics of Loops *)
+inductive while :: "'a cond \<Rightarrow> 'a prog \<Rightarrow> 'a prog" where
+while_baseI[intro]:
+  "\<lbrakk>\<not> t s\<rbrakk> \<Longrightarrow> while t B s s" |
+while_stepI[intro]:
+  "\<lbrakk>t s; B s s'; while t B s' s''\<rbrakk> \<Longrightarrow> while t B s s''"
+
+inductive prefix :: "'a cond \<Rightarrow> 'a prog \<Rightarrow> 'a prog" where
+prefix_baseI[intro]:
+  "prefix t B s s" |
+prefix_stepI[intro]:
+  "\<lbrakk>t s; B s s'; prefix t B s' s''\<rbrakk> \<Longrightarrow> prefix t B s s''"
+
+lemma prefix_while[intro]:
+  assumes "prefix t B s s'" "\<not> t s'"
+  shows  "while t B s s'"
+  using assms
+  by induction auto
+
+lemma prefix_step[intro]:
+  assumes "prefix t B s s'" "t s'" "B s' s''"
+  shows   "prefix t B s s''"
+  using assms
+  by induction auto
+
+(* Definition 2: Validity of Hoare-Triples (partial correctness *)
+inductive hoare :: "'a cond \<Rightarrow> 'a prog \<Rightarrow> 'a cond \<Rightarrow> bool" where
+hoareI[intro!]:
+"\<lbrakk>\<And> s s'. P s \<Longrightarrow> c s s' \<Longrightarrow> Q s'\<rbrakk>
+  \<Longrightarrow> hoare P c Q"
+
+lemma hoareE[elim]:
+  assumes "hoare P c Q"
+  assumes "P s" "c s s'"
+  obtains "Q s'"
+  using assms by (blast elim: hoare.cases)
+
+inductive invariant :: "'a cond \<Rightarrow> 'a cond \<Rightarrow> 'a cond \<Rightarrow> 'a prog \<Rightarrow> 'a cond \<Rightarrow> bool" where
+invariantI[intro!]:
+"\<lbrakk>\<And> s.    \<lbrakk>P s\<rbrakk> \<Longrightarrow> I s;
+  \<And> s s'. \<lbrakk>I s; t s; B s s'\<rbrakk> \<Longrightarrow> I s';
+  \<And> s.    \<lbrakk>I s; \<not> t s\<rbrakk> \<Longrightarrow> Q s\<rbrakk>
+  \<Longrightarrow> invariant P I t B Q"
+
+inductive_cases invariantE[elim]: "invariant P I t B Q"
+
+lemma invariant_last:
+  assumes "while t B s s'"
+  assumes "invariant P I t B Q"
+  assumes "I s"
+  shows   "\<not> t s'" "I s'"
+  using assms
+  by induction auto
+
+lemma invariant_correct:
+  assumes "while t B s s'"
+  assumes "invariant P I t B Q"
+  assumes "I s"
+  shows   "Q s'"
+  using assms
+  by induction auto
+
+corollary invariant_sound:
+  assumes "invariant P I t B Q"
+  shows   "hoare P (while t B) Q"
+proof
+  fix s s'
+  assume "P s"
+  with assms have "I s"
+    by blast
+  moreover assume "while t B s s'"
+  ultimately show "Q s'"
+    using assms by (metis invariant_correct)
+qed
+
+lemma invariant_complete:
+  assumes "hoare P (while t B) Q"
+  shows   "invariant P (\<lambda> s. \<exists> s0. P s0 \<and> prefix t B s0 s) t B Q"
+  using assms by blast
+
+inductive summary :: "'a cond \<Rightarrow> 'a cond \<Rightarrow> 'a prog \<Rightarrow> 'a rel \<Rightarrow> 'a cond \<Rightarrow> bool" where
+summaryI[intro!]:
+"\<lbrakk>\<And> s s'.     \<lbrakk>P s; \<not> t s'; R s s'\<rbrakk> \<Longrightarrow> Q s';
+  \<And> s s' s''. \<lbrakk>t s; B s s'; R s' s''\<rbrakk> \<Longrightarrow> R s s'';
+  \<And> s.        \<lbrakk>\<not> t s\<rbrakk> \<Longrightarrow> R s s\<rbrakk>
+  \<Longrightarrow> summary P t B R Q"
+
+inductive_cases summaryE[elim]: "summary P t R B Q"
+
+lemma summary_correct:
+  assumes "while t B s s'"
+  assumes "summary P t B R Q"
+  assumes "R s' s'"
+  shows   "R s  s'"
+  using assms
+  by induction auto
+
+lemma while_last[elim]:
+  assumes "while t B s s'"
+  shows   "\<not> t s'"
+  using assms
+  by induction auto
+
+lemma summary_sound:
+  assumes "summary P t B R Q"
+  shows   "hoare P (while t B) Q"
+proof
+  fix s s'
+  assume w: "while t B s s'"
+  then have t: "\<not> t s'" ..
+  with assms have R': "R s' s'"
+    by blast
+  with assms w have "R s s'"
+    by (metis summary_correct)
+  moreover assume "P s"
+  ultimately show "Q s'"
+    using assms t by blast
+qed
+
+lemma summary_complete:
+  assumes "hoare P (while t B) Q"
+  shows   "summary P t B (while t B) Q"
+  using assms by blast+
+
+lemma lift_summary:
+  assumes "summary   P t B R Q"
+  shows   "invariant P (\<lambda> s. \<exists> s0. P s0 \<and> (\<forall> sn. R s sn \<longrightarrow> R s0 sn)) t B Q"
+  using assms by blast+
+
+lemma lift_invariant:
+  assumes "invariant P I t B Q"
+  shows   "summary   P t B (\<lambda> s s'. I s \<longrightarrow> \<not> t s' \<and> I s') Q"
+  using assms by auto
+
+lemma lift_invariant':
+  assumes "invariant P I t B Q"
+  shows   "summary   P t B (\<lambda> s s'. I s \<longrightarrow> Q s') Q"
+  using assms by auto
+
+lemma strengthen_invariant:
+  assumes "invariant P I t B Q"
+  shows   "invariant P (\<lambda> s. \<exists> s0. P s0 \<and> I s) t B Q"
+  using assms by blast
+
+inductive functional :: "'a cond \<Rightarrow> 'a prog \<Rightarrow> ('a \<Rightarrow> 'a) \<Rightarrow> bool" where
+"\<lbrakk>\<And> s sn. while t B s sn = (sn = f s)\<rbrakk>
+  \<Longrightarrow> functional t B f"
+
+inductive_cases functionalE[elim]: "functional t B f"
+
+lemma functional_correct:
+  assumes "functional t B f"
+  assumes "\<And> s. P s \<Longrightarrow> Q (f s)"
+  shows   "hoare P (while t B) Q"
+  using assms by auto
+
+lemma functional_confluence:
+  assumes "functional t B f"
+  assumes "while t B s  sn"
+  assumes "while t B s' sn"
+  shows   "f s = f s'"
+  using assms by auto
+
+lemma functional_exit[simp]:
+  assumes "functional t B f"
+  assumes "\<not> t sn"
+  shows   "f sn = sn"
+  using assms
+  by (metis functionalE while_baseI)
+
+lemma functional_step[simp]:
+  assumes "functional t B f"
+  assumes "t s" "B s s'"
+  shows   "f s = f s'"
+proof -
+  from assms(1)   have w': "while t B s' (f s')" by blast
+  with assms(2,3) have w:  "while t B s  (f s')" by rule
+  from assms(1) w w'
+  show ?thesis
+    by (rule functional_confluence) (* or directly by auto *)
+qed
+
+lemma functional_invariant:
+  assumes "functional t B f"
+  assumes "\<And> s. P s \<Longrightarrow> Q (f s)"
+  shows   "invariant P (\<lambda> s. \<exists> s0. P s0 \<and> f s = f s0) t B Q"
+  using assms by auto
+
+lemma functional_summary:
+  assumes "functional t B f"
+  assumes "\<And> s. P s \<Longrightarrow> Q (f s)"
+  shows   "summary P t B  (\<lambda> s sn. \<not> t sn \<and> sn = f s) Q"
+  using assms by auto
+
+lemma functional_correspondence:
+  assumes "functional t B f"
+  shows   "invariant P (\<lambda> s. \<exists> s0. P s0 \<and> f s = f s0) t B Q
+       \<longleftrightarrow> summary P t B (\<lambda> s sn. \<not> t sn \<and> f sn = f s) Q"
+  using assms by auto
+
+fun ack :: "[nat,nat] \<Rightarrow> nat" where
+  "ack 0 n             = Suc n"
+| "ack (Suc m) 0       = ack m 1"
+| "ack (Suc m) (Suc n) = ack m (ack (Suc m) n)"
+
+fun acklist :: "nat list \<Rightarrow> nat" where
+  "acklist (n#m#L) = acklist (ack m n # L)"
+| "acklist [m] = m"
+
+inductive TEST :: "nat list \<Rightarrow> bool" where
+"TEST (n#m#L)"
+
+lemma not_TEST[simp]: "(\<not> TEST L) = (L = [] \<or> (\<exists> n. L = [n]))"
+  unfolding TEST.simps
+  apply auto
+  apply (case_tac L)
+  apply simp_all
+  apply (case_tac list)
+  by simp_all
+
+inductive STEP :: "nat list \<Rightarrow> nat list \<Rightarrow> bool" where
+"STEP (n#0#L)          (Suc n#L)" |
+"STEP (0#Suc m#L)      (1#m#L)" |
+"STEP (Suc n# Suc m#L) (n#Suc m#m#L)"
+
+lemma STEPs:
+  assumes "TEST L"
+  shows   "\<exists>! L'. STEP L L'"
+  using assms
+  apply (elim TEST.cases)
+  apply (simp add: STEP.simps)
+  apply (case_tac "m")
+  apply auto
+  apply (case_tac "n")
+   apply auto
+  done
+
+definition "ACK \<equiv> while TEST STEP"
+definition "INV s0 s \<equiv> s \<noteq> [] \<and> acklist s0 = acklist s"
+
+(* "ackloop_dom (ack m n # L) \<Longrightarrow> ackloop_dom (n # m # L)" *)
+
+definition "SM s s'  \<equiv> s \<noteq> [] \<longrightarrow> s' = [acklist s]"
+
+lemma ACK_INV:
+  "hoare (\<lambda> s. s = [n,m]) ACK (\<lambda> s'. s' = [ack m n])"
+  unfolding ACK_def
+proof (rule invariant_sound)
+  show "invariant (\<lambda>s. s = [n, m]) (INV [n, m]) TEST STEP (\<lambda>s'. s' = [ack m n])"
+  proof (rule, goal_cases)
+    case (1 s)
+    then show ?case
+      unfolding INV_def by simp
+  next
+    case (2 s s')
+    then show ?case
+      unfolding INV_def
+      by (auto elim!: STEP.cases)
+  next
+    case (3 s)
+    then show ?case
+      unfolding INV_def by auto
+  qed
+qed
+
+lemma ACK_SM:
+  "hoare (\<lambda> s. s = [n,m]) ACK (\<lambda> s'. s' = [ack m n])"
+  unfolding ACK_def
+proof (rule summary_sound)
+  show "summary (\<lambda>s. s = [n, m]) TEST STEP SM (\<lambda>s'. s' = [ack m n])"
+  proof (rule, goal_cases)
+    case (1 s s')
+    then show ?case
+      unfolding SM_def by auto
+  next
+    case (2 s s' s'')
+    then show ?case
+      unfolding SM_def
+      by (auto elim!: STEP.cases)
+  next
+    case (3 s)
+    then show ?case
+      unfolding SM_def by auto
+  qed
+qed
+
+
+inductive test :: "('a * 'b) cond \<Rightarrow> ('a * 'b) prog \<Rightarrow> ('a * 'b \<Rightarrow> 'a) \<Rightarrow> bool" where
+"(\<And> x y x' y'. while t B (x,y) (x',y') \<Longrightarrow> x' = f(x,y))
+  \<Longrightarrow> test t B f"
+
+inductive_cases testE[elim]: "test t B f"
+
+lemma test_exit[simp]:
+  assumes "test t B f"
+  assumes "\<not> t (x,y)"
+  shows   "f (x,y) = x"
+  using assms
+  by (metis testE while_baseI)
+
+lemma test_step[simp]:
+  assumes "test t B f"
+  assumes "t (x,y)" "B (x,y) (x',y')" "while t B (x',y') (x'',y'')"
+  shows   "f (x,y) = f (x',y')"
+proof -
+
+end
