isabelle/Unary.thy
@@ -1,0 +1,79 @@
+theory Unary
+  imports Summaries
+begin
+
+inductive usummary_correct :: "'a cond \<Rightarrow> 'a cond \<Rightarrow> 'a prog \<Rightarrow> 'a cond \<Rightarrow> 'a cond \<Rightarrow> bool" where
+usummary_correctI[intro!]:
+"\<lbrakk>\<And> s s'. \<lbrakk>P s; R s\<rbrakk> \<Longrightarrow> Q s';
+  \<And> s.    \<lbrakk>\<not> t s\<rbrakk> \<Longrightarrow> R s;
+  \<And> s.    \<lbrakk>  t s; B s Err\<rbrakk> \<Longrightarrow> R s;
+  \<And> s s'. \<lbrakk>  t s; B s (Brk s')\<rbrakk> \<Longrightarrow> R s;
+  \<And> s s'. \<lbrakk>  t s; B s (Ok  s'); R s'\<rbrakk> \<Longrightarrow> R s\<rbrakk>
+  \<Longrightarrow> usummary_correct P t B R Q"
+
+inductive_cases usummary_correctE[elim]: "usummary_correct P t B Q R"
+
+lemma usummary_post:
+  assumes "while t B s r"
+  assumes "r = Ok s'"
+  assumes "usummary_correct P t B R Q"
+  assumes "P s"
+  shows   "Q s'"
+proof -
+  from assms(1-3) have "R s"
+    by induction blast+
+  with assms(3,4) show ?thesis
+    by blast
+qed
+
+theorem usummary_complete:
+  assumes "correct P (while t B) Q"
+  obtains R where "usummary_correct P t B R Q"
+proof -
+  have "usummary_correct P t B (\<lambda> s. Q s \<and> (\<forall> s'. suffix t B s s' \<longrightarrow> Q s')) Q"
+  proof (rule, goal_cases)
+    case (1 s s')
+    then show ?case
+      using assms
+      sorry
+  next
+    case (2 s)
+    then show ?case
+      using assms try
+      sorry
+  next
+    case (3 s)
+    then show ?case sorry
+  next
+    case (4 s s')
+    then show ?case sorry
+  next
+    case (5 s s')
+    then show ?case sorry
+  qed
+  then show ?thesis ..
+qed
+
+theorem summary_unary:
+  assumes "summary_correct  P t B R Q"
+  shows   "usummary_correct P t B (\<lambda> s. \<forall> sn. R s sn) Q"
+proof (rule, goal_cases)
+  case (1 s s')
+  then show ?case
+    using assms by blast
+next
+  case (2 s)
+  then show ?case
+    using assms sorry
+next
+  case (3 s)
+  then show ?case sorry
+next
+  case (4 s s')
+  then show ?case sorry
+next
+  case (5 s s')
+  then show ?case sorry
+qed
+
+end
